theory/Proof1.thy
@@ -23,59 +23,11 @@ lemma list_in_list_prop:"list_in_list l 0 l"
   using list_in_list_prop_aux1
   by (metis append_Nil list_in_list_prop_aux2 list.size(3))
 
-lemma x64_encode_decode_consistency:
- "list_in_list l_bin pc l \<Longrightarrow>
+
+axiomatization where x64_encode_decode_consistency: 
+  "list_in_list l_bin pc l \<Longrightarrow>
   l_bin = x64_encode ins \<Longrightarrow>
   length l_bin = n \<Longrightarrow>
-   x64_decode pc l = Some (n, ins)"
-  sorry
-  (*using list_in_list_prop
-  apply(cases ins,simp_all)
-  subgoal for dst src 
-    \<comment> \<open> Paddq_rr \<close> 
-    apply (unfold Let_def construct_rex_to_u8_def construct_modsib_to_u8_def)
-    subgoal apply (cases src; simp;cases dst; auto simp add: x64_decode_def bitfield_insert_u8_def Let_def ireg_of_u8_def
-          Suc3_eq_add_3 add.commute)
-      done
-    done
-   apply(unfold x64_decode_def;auto)
-  subgoal for dst
-    apply (unfold Let_def construct_rex_to_u8_def construct_modsib_to_u8_def)
- subgoal by (cases dst; auto simp add: x64_decode_def bitfield_insert_u8_def Let_def ireg_of_u8_def)
-  done
-  defer
- subgoal for dst src
-  \<comment> \<open> Pmovq_rr \<close> 
-   apply (unfold Let_def construct_rex_to_u8_def construct_modsib_to_u8_def)
-   (*apply(erule conjE; erule conjE)*)
-   subgoal by (cases src; cases dst; auto simp add: x64_decode_def bitfield_insert_u8_def Let_def ireg_of_u8_def)
-    done
-  subgoal for dst 
-    \<comment> \<open> Pmulq_r \<close> 
-    apply (unfold Let_def construct_rex_to_u8_def construct_modsib_to_u8_def)
-    subgoal by (cases dst; auto simp add: x64_decode_def bitfield_insert_u8_def Let_def ireg_of_u8_def)
-    done
-  subgoal for dst
-    \<comment> \<open> Ppopl_i \<close> 
-    apply (unfold Let_def construct_rex_to_u8_def construct_modsib_to_u8_def)
-    apply (cases dst; auto simp add: x64_decode_def bitfield_insert_u8_def Let_def ireg_of_u8_def)
-  done
-  done*)
-
-(*lemma x64_encodes_decodes_consistency:
-  "Some l_bin = x64_encodes2 ins \<Longrightarrow>
-    x64_decodes 0 l_bin = Some ins_list \<Longrightarrow>
-    map snd ins_list = ins" 
-  sorry*)
-(*
-value "x64_decode 0 [0b01001000,0b00000001,0b11011000]"
-value "x64_decodes_aux 0 [0xc3,0b01001000,0b00000001,0b11011000]"
-value "x64_decodes 0 [0xc3,0b01001000,0b00000001,0b11011000]"
-value "x64_decode 1 [0xc3,0b01001000,0b00000001,0b11011000]"
-value "x64_encodes_suffix []"
-value "x64_decodes 0 []"*)
-
-
-
+  x64_decode pc l = Some (n, ins)"
 
 end
